language_formalisation/substitution/substitution.v
@@ -1,5 +1,5 @@
-Add LoadPath "C:\Users\Ziga\Documents\Ziga_podatki\PHD\language_formalisation\syntax".
-(* Add Rec LoadPath "E:\Ziga_Podatki\faks\PHD\language_formalisation\syntax". *)
+(* Add LoadPath "C:\Users\Ziga\Documents\Ziga_podatki\PHD\language_formalisation\syntax". *)
+Add LoadPath "E:\Ziga_Podatki\faks\PHD\language_formalisation\syntax".
 Require Export syntax Arith.
 Require Import Le Compare_dec.
 
