language_formalisation/syntax/syntax_lemmas.v
@@ -1,0 +1,71 @@
+(* Add LoadPath "C:\Users\Ziga\Documents\Ziga_podatki\PHD\language_formalisation\syntax". *)
+Add LoadPath "E:\Ziga_Podatki\faks\PHD\language_formalisation\syntax".
+Require Export Arith syntax.
+Require Import Le Compare_dec.
+
+Lemma gets_same Γ (id:var_id) (db_i:nat) :
+  id_has_dbi id db_i = true -> get_vtype Γ id = get_vtype_i Γ db_i.
+Proof.
+revert id db_i. induction Γ; intros id db_i matches; destruct id as (name, num).
++ auto.
++ simpl in matches. apply beq_nat_true in matches.
+  rewrite matches. simpl. auto.
+Qed.
+
+Lemma get_in_changed_other Γ j k αj :
+  j <> k -> get_vtype_i Γ k = get_vtype_i (ctx_change_var Γ j αj) k.
+Proof.
+revert j k. induction Γ; intros j k neq_jk.
+auto.
+simpl.
+destruct k.
++ destruct j; auto.
+  apply beq_nat_false_iff in neq_jk. simpl in neq_jk. discriminate.
++ destruct j; auto.
+  simpl. apply IHΓ. omega.
+Qed.
+
+Lemma get_in_changed_same Γ j αj_orig αj 
+  (p_j : get_vtype_i Γ j = Some αj_orig) :
+  get_vtype_i (ctx_change_var Γ j αj) j = Some αj.
+Proof.
+revert j p_j. induction Γ; intros j p_j.
++ simpl in p_j. discriminate.
++ destruct j; auto. simpl.
+  apply IHΓ. simpl in p_j. assumption.
+Qed.
+
+Lemma get_in_switched_other Γ k i j αi αj
+  (p_i : get_vtype_i Γ i = Some αi) (p_j : get_vtype_i Γ j = Some αj) :
+  i <> k -> j <> k ->
+  get_vtype_i Γ k = get_vtype_i (ctx_switch_vars Γ i j αi αj p_i p_j) k.
+Proof.
+revert k i j p_i p_j. induction Γ;
+intros k i j p_i p_j neq_ik neq_jk.
+auto.
+revert i j p_i p_j neq_ik neq_jk. destruct k;
+intros i j p_i p_j neq_ik neq_jk.
++ destruct i.
+  - apply beq_nat_false_iff in neq_ik. simpl in neq_ik. discriminate.
+  - simpl. destruct j; auto.
+    apply beq_nat_false_iff in neq_jk. simpl in neq_jk. discriminate.
++ destruct i.
+  - destruct j; auto.
+    simpl. apply get_in_changed_other. omega.
+  - destruct j; simpl.
+    * apply get_in_changed_other. omega.
+    * unfold ctx_switch_vars in IHΓ. apply IHΓ.
+      auto. auto. omega. omega.
+Qed.
+      
+Lemma get_in_switched_i Γ i j αi αj
+  (p_i : get_vtype_i Γ i = Some αi) (p_j : get_vtype_i Γ j = Some αj) :
+  get_vtype_i Γ i = get_vtype_i (ctx_switch_vars Γ i j αi αj p_i p_j) j.
+Proof.
+revert i j p_i p_j. induction Γ; intros i j p_i p_j.
+auto.
+destruct i; destruct j; auto; simpl.
++ apply eq_sym. simpl in p_i. rewrite p_i.
+  apply (get_in_changed_same Γ j αj). auto.
++ unfold ctx_switch_vars in IHΓ. apply IHΓ. auto. auto.
+Qed.
