language_formalisation/type_system/type_aux_lemmas.v
@@ -1,0 +1,111 @@
+(* Add LoadPath "C:\Users\Ziga\Documents\Ziga_podatki\PHD\language_formalisation\syntax". *)
+(* Add LoadPath "C:\Users\Ziga\Documents\Ziga_podatki\PHD\language_formalisation\type_system". *)
+(* Add LoadPath "C:\Users\Ziga\Documents\Ziga_podatki\PHD\language_formalisation\substitution". *)
+(* Add LoadPath "C:\Users\Ziga\Documents\Ziga_podatki\PHD\language_formalisation\operational_semantics". *)
+Add LoadPath "E:\Ziga_Podatki\faks\PHD\language_formalisation\syntax".
+Add LoadPath "E:\Ziga_Podatki\faks\PHD\language_formalisation\type_system".
+Add LoadPath "E:\Ziga_Podatki\faks\PHD\language_formalisation\substitution".
+Add LoadPath "E:\Ziga_Podatki\faks\PHD\language_formalisation\operational_semantics".
+
+Require Export syntax bidirectional substitution Omega Logic.
+
+Ltac inv H := inversion H; clear H; subst.
+
+(* Switch lemmas *)
+Lemma v_switch_safe
+  (Γ:ctx) i (αi:vtype) j (αj:vtype) (v:val) (A:vtype)
+  (p_i : get_vtype_i Γ i = Some αi) (p_j : get_vtype_i Γ j = Some αj) :
+  vcheck Γ v A ->
+  vcheck (ctx_switch_vars Γ i j αi αj p_i p_j) (v_switch_vars v i j) A
+
+with c_switch_safe 
+  (Γ:ctx) i (αi:vtype) j (αj:vtype) (c:comp) (C:ctype)
+  (p_i : get_vtype_i Γ i = Some αi) (p_j : get_vtype_i Γ j = Some αj) :
+  ccheck Γ c C -> 
+  ccheck (ctx_switch_vars Γ i j αi αj p_i p_j) (c_switch_vars c i j) C
+
+with h_switch_safe
+  (Γ:ctx) i (αi:vtype) j (αj:vtype) (h:hcases) (Σ:sig) (D:ctype)
+  (p_i : get_vtype_i Γ i = Some αi) (p_j : get_vtype_i Γ j = Some αj) :
+  hcheck Γ h Σ D ->
+  hcheck (ctx_switch_vars Γ i j αi αj p_i p_j) (h_switch_vars h i j) Σ D.
+Proof.
+{
+clear v_switch_safe.
+revert Γ i j αi αj A p_i p_j; induction v;
+intros Γ i j αi αj A p_i p_j orig; simpl.
+{ (* relevant case *)
+  destruct v as (num, name).
+  inv orig. inv H.
+  remember (name =? i) as cmpi.
+  induction cmpi.
+  + apply CheckVBySynth. apply SynthVar. simpl.
+    simpl in H2. rewrite <-Heqcmpi in H2. assumption.
+  + remember (name =? 1) as cmpj.
+    induction cmpj.
+    * apply CheckVBySynth. apply SynthVar. simpl.
+      simpl in H2. rewrite <-Heqcmpi in H2.
+      apply eq_sym in Heqcmpj.
+      apply beq_nat_true in Heqcmpj. rewrite Heqcmpj in H2. simpl in H2.
+      assumption.
+    * apply CheckVBySynth. apply SynthVar. simpl.
+      rewrite <-Heqcmpi. simpl.
+      simpl in H2. rewrite <-Heqcmpi in H2.
+      apply eq_sym in Heqcmpi. apply eq_sym in Heqcmpj.
+      apply beq_nat_false in Heqcmpi. apply beq_nat_false in Heqcmpj.
+      assert (name-1 <> 0) by omega.
+      apply beq_nat_false_iff in H. rewrite H. rewrite H in H2. simpl.
+      assumption.
+}
+all: inv orig; try inv H; simpl.
++ apply CheckVBySynth. apply SynthUnit.
++ apply CheckVBySynth. apply SynthInt.
++ apply CheckInl. apply IHv. assumption.
++ apply CheckInr. apply IHv. assumption.
++ apply CheckPair; apply IHv1 || apply IHv2; apply CheckVBySynth; assumption.
++ apply CheckPair; apply IHv1 || apply IHv2; assumption.
++ apply CheckFun. 
+
+}
+
+
+
+
+(* Other lemmas *)
+Lemma v_add_to_ctx_safe (Γ:ctx) (α:vtype) (v:val) (A:vtype) :
+  vcheck Γ v A ->
+  vcheck (CtxU Γ α) (Sub.v_shift v 1 0) A
+  /\
+  v_no_var_j v j
+with c_add_to_ctx_safe (Γ:ctx) (α:vtype) (c:comp) (C:ctype) :
+  ccheck Γ c C -> ccheck (CtxU Γ α) (Sub.c_shift c 1 0) C
+with h_add_to_ctx_safe (Γ:ctx) (α:vtype) (h:hcases) (Σ:sig) (D:ctype) :
+  hcheck Γ h Σ D -> hcheck (CtxU Γ α) (Sub.h_shift h 1 0) Σ D.
+Proof.
+all:
+rename v_add_to_ctx_safe into v_lemma;
+rename c_add_to_ctx_safe into c_lemma;
+rename h_add_to_ctx_safe into h_lemma.
+{
+clear v_lemma.
+revert Γ α A. induction v; intros Γ α A orig; simpl.
++ inv orig. inv H. apply CheckVBySynth. apply SynthVar.
+  destruct v as (name, num). simpl.
+  assert (num + 1 =? 0 = false).
+  { apply beq_nat_false_iff. omega. }
+  rewrite H. assert (num+1-1=num) by omega.
+  rewrite H0. auto.
++ inv orig. inv H. apply CheckVBySynth. apply SynthUnit.
++ inv orig. inv H. apply CheckVBySynth. apply SynthInt.
++ inv orig. inv H. apply CheckInl. apply IHv. assumption.
++ inv orig. inv H. apply CheckInr. apply IHv. assumption.
++ inv orig. inv H.
+  - apply CheckPair.
+    * apply IHv1. apply CheckVBySynth. assumption. 
+    * apply IHv2. apply CheckVBySynth. assumption.
+  - apply CheckPair.
+    * apply IHv1. assumption. 
+    * apply IHv2. assumption.
++ inv orig. inv H. apply CheckFun. apply c_lemma.  
+
+}
